# Induction Proof for Eq. (4)

**Provided:**

$$F_n=\begin{cases}
0, & n=0 \\
1, & n = 1 \\
F_{n-1}+F_{n-2}, & n \ge 2
\end{cases}$$

**Prove**: $F_{n+1}F_{n-1}-F_{n}^{2}=(-1)^n, \, n \ge 1$.

***Proof:***

1. **Base Case:**
   
    It is true when $n = 1$, since $F_{n+1}F_{n-1}-F_{n}^{2}=F_{2}F_{0}-F_{1}^{2}=1\times 0-1^2=-1=(-1)^{1}$.
2. **Induction Hypothesis:**
   
    Assume the statement is true for some $n = k \ge 1$:
   
    $$F_{k+1}F_{k-1}-F_{k}^2 = (-1)^k$$
3. **Induction Step:**
   
    For $n=k+1$, 

$$\begin{aligned} F_{k+2}F_{k}-F_{k+1}^{2} & = (F_{k}+F_{k+1})F_{k}-F_{k+1}^{2}\\
                        & = F_{k}^{2}+F_{k}F_{k+1}-F_{k+1}^2 \\
                        & = F_{k}^{2} + F_{k+1}(F_{k}-F_{k+1}) \\
                        & = F_{k}^2+F_{k+1}(F_{k+1}-F_{k-1}-F_{k+1}) \\
                        & = F_{k}^{2} - F_{k+1}F_{k-1} \\
                        & = -(F_{k+1}F_{k-1}-F_{k}^{2}) \\
                        & = - (-1)^k \\
                        & = (-1)^{k+1} \end{aligned}$$

Therefore, the statement also holds for $n=k+1$.

So we have proved that $F_{n+1}F_{n-1}-F_{n}^{2}=(-1)^n$ is true for all $n \ge 1$.


